Logic.v
@@ -2,107 +2,75 @@ Require Import ACTL.
 Require Import EDEN.
 Require Import Coq.Setoids.Setoid.
 
-
-
+  
 Set Implicit Arguments.
 
 
-
-Notation "s |= f" := (@sat State action Trans f s)(at level 80).
-Notation "|= f" := (forall s, s |= f)(at level 80).
-Notation τ := (action_ tau).
-Notation "< chi > f" := (E (⊤ [τ] U [chi] f))(at level 50, chi at level 5).
-Notation "[ chi ] f" := (¬ <chi> ¬ f)(at level 50, chi at level 5).
-Notation "'EX' f" := (<any> f)(at level 50).
-Notation "'AX' f" := ([any] f)(at level 50).
-Notation "'EF' f" := (f ∨ EF [any] f)(at level 50).
-Notation "'AF' f" := (f ∨ AF [any] f)(at level 50).
-Notation "'EG' f" := (¬ AF ¬ f)(at level 50).
-Notation "'AG' f" := (¬ EF ¬ f)(at level 50).
+Definition lts := Build_LTS State Action Trans tau Tau_eq.
 
 
-Notation "f 'EU' f'" := (f' ∨ (f ∧ (EX (E (f U f')))))(at level 50).
-Notation "f 'AU' f'" := (f' ∨ (f ∧ (AX (A (f U f')))))(at level 50).
-Notation "f 'EW' f'" := (¬ ((¬ f') AU ((¬ f) ∧ (¬ f'))))(at level 50).
-Notation "f 'AW' f'" := (¬ ((¬ f') EU ((¬ f) ∧ (¬ f'))))(at level 50).
+Notation Path := (@path lts).
+Notation Form := (@form lts).
+Notation Formr := (@formr lts).
+Notation Citizen := (citizen env).
+Notation Admin := (admin env).
+Notation Var := (var env).
 
-Notation Path := (@path State action Trans).
-Notation Form := (@form action).
-Notation Formr := (@formr action).
-
-Notation Action_ := (@action_ action).
-Notation Act_var := (@act_var Proposal).
+Notation State := (@ACTL.state lts).
+Notation Action_ := (@ACTL.action_ lts).
+Notation Tau := (@ACTL.tau lts).
+Notation Act_var := (@act_var env).
 
 
 (* 命題変数 *)
 Notation HasNoBudget adm := (<(Action_ (Act_var (hasNoBudget adm)))> ⊤).
 Notation HasNoComitee adm := (<(Action_ (Act_var (hasNoComitee adm)))> ⊤).
-Notation HasNoTenureWoker adm := (<(Action_ (Act_var (hasNoTenureWoker adm)))> ⊤).
-Notation HasNoMember adm := (<(Action_ (Act_var (hasNoMember adm)))> ⊤).
 Notation IsBudgetRestricted adm := (<(Action_ (Act_var (isBudgetRestricted adm)))> ⊤).
 Notation IsTransferRestricted adm := (<(Action_ (Act_var (isBudgetRestricted adm)))> ⊤).
 Notation IsAssignmentRestrected adm adm' := (<(Action_ (Act_var (isAssignmentRestrected adm adm')))> ⊤).
-Notation IsAdminControlRestricted adm := (<(Action_ (Act_var (isAdminControlRestricted adm)))> ⊤).
+Notation IsAdminControlRestricted adm := (<(Action_ (Act_var (isadminControlRestricted adm)))> ⊤).
 Notation IsAssigned adm ctz := (<(Action_ (Act_var (isAssigned adm ctz)))> ⊤).
 Notation IsProposed adm prp := (<(Action_ (Act_var (isProposed adm prp)))> ⊤).
-Notation IsTenureWorker adm ctz := (<(Action_ (Act_var (isTenureWorker adm ctz)))> ⊤).
-Notation IsWithinExpiration adm ctz := (<(Action_ (Act_var (isWithinExpiration adm ctz)))> ⊤).
 
 
-Notation Propose prp := (Action_ (act_proposal prp)).
+
+Notation Propose prp := (Action_ (act_propose prp)).
 Notation Withdraw adm n := (Propose (withdraw adm n)).
 Notation Deposit adm n := (Propose (deposit adm n)).
 Notation Transfer from to n := (Propose (transfer from to n)).
-Notation AssignMember adm n := (Propose (assignMember adm n)).
-Notation DismissalMember adm n := (Propose (dismissalMember adm n)).
+Notation AssignMember adm n := (Propose (assign adm n)).
+Notation DismissalMember adm n := (Propose (dismissal adm n)).
 Notation AssignTenureWorker adm n := (Propose (withdraw adm n)).
-Notation DismissalTenureWorker adm n := (Propose (dismissalTenureWorker adm n)).
 Notation GenAdmin adm n := (Propose (genAdmin adm n)).
 Notation SlashAdmin adm n := (Propose (slashAdmin adm n)).
 
 Notation Deliberate adm := (Action_ (act_deliberate adm)).
 
 
-Definition ROOT := Adm 0.
-Definition PROFESSIONALS := Adm 1.
-Definition FACILITATORS := Adm 2.
-Definition REGISTRATOR := Adm 3.
-Definition POLICE := Adm 4.
-(* Definition JUDICIARY := Adm 5.
-Definition MILITARY := Adm 6.
-Definition MEDIA := Adm 7.
-Definition EDUCATION := Adm 8. *)
+
+Variable ROOT PROFESSIONALS FACILITATORS REGISTRATOR DUMMY : Admin.
 
 
 Definition IsAssignmentRestrectedStrict adm :=
     IsAssignmentRestrected adm ROOT ∧
     IsAssignmentRestrected adm PROFESSIONALS ∧
     IsAssignmentRestrected adm FACILITATORS ∧
-    IsAssignmentRestrected adm POLICE.
-    (* IsAssignmentRestrected adm JUDICIARY ∧
-    IsAssignmentRestrected adm MILITARY ∧   
-    IsAssignmentRestrected adm MEDIA ∧   
-    IsAssignmentRestrected adm EDUCATION. *)
-
-
+    IsAssignmentRestrected adm DUMMY.
 
 
 
 Definition ROOT_spec :=
     IsBudgetRestricted ROOT ∧
-    HasNoTenureWoker ROOT ∧
     IsAssignmentRestrected ROOT ROOT.
 
     
 Definition PROFESSIONAL_spec :=
     HasNoBudget PROFESSIONALS ∧
-    HasNoComitee PROFESSIONALS ∧
-    HasNoMember PROFESSIONALS.
+    HasNoComitee PROFESSIONALS.
 
 Definition FACILITATORS_spec :=
     HasNoBudget FACILITATORS ∧
-    HasNoComitee FACILITATORS ∧
-    HasNoMember FACILITATORS.
+    HasNoComitee FACILITATORS.
 
     
 Definition REGISTRATOR_spec :=
@@ -112,85 +80,55 @@ Definition REGISTRATOR_spec :=
     IsAssignmentRestrected REGISTRATOR REGISTRATOR ∧
     IsAssignmentRestrected REGISTRATOR FACILITATORS ∧
     IsAssignmentRestrected REGISTRATOR REGISTRATOR ∧
-    IsAssignmentRestrected REGISTRATOR POLICE.
+    IsAssignmentRestrected REGISTRATOR DUMMY.
 
-Definition POLICE_spec :=
-    IsBudgetRestricted POLICE ∧
-    IsTransferRestricted POLICE ∧
-    IsAdminControlRestricted POLICE ∧
-    IsAssignmentRestrected POLICE ROOT ∧
-    IsAssignmentRestrected POLICE PROFESSIONALS ∧
-    IsAssignmentRestrected POLICE FACILITATORS ∧
-    IsAssignmentRestrected POLICE REGISTRATOR ∧
-    IsAssignmentRestrected POLICE POLICE.
+Definition DUMMY_spec :=
+    IsBudgetRestricted DUMMY ∧
+    IsTransferRestricted DUMMY ∧
+    IsAdminControlRestricted DUMMY ∧
+    IsAssignmentRestrected DUMMY ROOT ∧
+    IsAssignmentRestrected DUMMY PROFESSIONALS ∧
+    IsAssignmentRestrected DUMMY FACILITATORS ∧
+    IsAssignmentRestrected DUMMY REGISTRATOR ∧
+    IsAssignmentRestrected DUMMY DUMMY.
 
 
 Definition SPEC :=
-    ROOT_spec ∧ PROFESSIONAL_spec ∧ REGISTRATOR_spec ∧ POLICE_spec.
+    ROOT_spec ∧ PROFESSIONAL_spec ∧ REGISTRATOR_spec ∧ DUMMY_spec.
 
-Ltac  satisfy := unfold sat; fold (sat (trans := Trans)).
+Ltac  satisfy := unfold sat; fold (@sat lts).
 
-Theorem tau_eq : forall  s s', Trans s tau s' <->  s = s'.
-Proof.
-    intros s s'; split; intro H; symmetry; auto.    
-Qed.
+
 
 Theorem IsAssignedUnfdold adm c s :
     s |= IsAssigned adm c  <-> 
-        match Ssubstate s adm with 
+        match s adm with 
         | None => False 
-        | Some ss' => c \in SSmember ss'
+        | Some ss' => c \in memberSS ss'
         end.
 Proof.
     split; satisfy; intro H.
     -   induction H as [r [Hr [_ HU]]].
         induction HU; simpl in *; subst; auto; simpl in *.
-        +   destruct r, p; simpl in *; subst;
-                inversion t; subst; destruct s'; auto.
+        +   destruct r, p; simpl in *; subst; inversion t; subst; simpl in *; auto.                
         +   apply IHHU; auto.
-    -   remember (Ssubstate s adm) as ss.
+    -   remember (s adm) as ss.
         destruct ss.
         +   assert (Trans s (Act_var (isAssigned adm c)) s) as Ht.
-            { constructor; simpl; destruct (Ssubstate s adm);
+            { constructor; simpl; destruct (s adm);
                 inversion Heqss; subst; auto.
             }    
-            Check path.
-
             exists (Run s (nilp s (Act_var (isAssigned adm c)) s Ht));
             repeat split; constructor; unfold sata; auto.
         +   inversion H.
 Qed.
 
-Theorem IsProposedUnfold adm prp s : 
-            s |= IsProposed adm prp <->
-                match Ssubstate s adm with 
-                | None => False 
-                | Some ss => match SScomitee ss with
-                    | None => False 
-                    | Some cmt => prp =  Dproposal cmt
-                    end
-                end.
-Proof.
-    split; satisfy; intro H.
-    -   induction H as [r [Hr [_ HU]]].
-        induction HU; simpl in *; subst; auto; simpl in *.
-        +   destruct r, p; simpl in *; subst;
-                inversion t; subst; destruct s'; auto.
-        +   apply IHHU; auto.
-    -   remember (Ssubstate s adm) as ss.
-        destruct ss.
-        +   assert (Trans s (Act_var (isProposed adm prp)) s) as Ht.
-            { constructor; simpl; destruct (Ssubstate s adm);
-                inversion Heqss; subst; auto.
-            }            
-            exists (Run s (nilp s (Act_var (isProposed adm prp)) s Ht));
-            repeat split; constructor; unfold sata; auto.
-        +   inversion H.
-Qed.            
+
+        
 
             
 Definition dismissible adm c :=
-    (IsProposed ROOT (dismissalMember adm c)) ∧ ¬ [Deliberate ROOT] (IsAssigned adm c).
+    (IsProposed ROOT (dismissal adm c)) ∧ ¬ [Deliberate ROOT] (IsAssigned adm c).
 
     
 Definition deliberate_soundness adm c :=
